@prefix dcterms: <http://purl.org/dc/terms/> .
@prefix owl: <http://www.w3.org/2002/07/owl#> .
@prefix prov: <http://www.w3.org/ns/prov#> .
@prefix rdf: <http://www.w3.org/1999/02/22-rdf-syntax-ns#> .
@prefix rdf: <http://xmlns.com/foaf/0.1/>.
@prefix rdfs: <http://www.w3.org/2000/01/rdf-schema#> .
@prefix skos: <http://www.w3.org/2004/02/skos/core#> .
@prefix uiote: <http://www.w3id.org/urban-iot/electric#> .
@prefix vann: <http://purl.org/vocab/vann/> .
@prefix xsd: <http://www.w3.org/2001/XMLSchema#> .
@prefix role: <https://w3id.org/omega-x/EnergyRoleOntology/>.
@prefix foaf: <http://xmlns.com/foaf/0.1/>.
@base  <https://w3id.org/omega-x/ontology/EnergyRole/>.
@prefix role: <https://w3id.org/omega-x/ontology/EnergyRole> .

<https://w3id.org/omega-x/ontology/EnergyRole/> a owl:Ontology ;
    dcterms:title "Energy Role Ontology"@en ;
    dcterms:description """Purpose: The Energy Role ontology is dedicated to business parties, their intended behaviour, and relationships with other elements involved in energy market business processes.
        Scope: The Energy Role ontology defines three generic concepts: business parties (participant), business roles (role), and their relationships (association). Roles are further refined in classifications specific to electromobility, flexibility, and local energy communities domains.
    """@en ;
    dcterms:issued "2024-05-06"^^xsd:date ;
    dcterms:modified "2024-05-03"^^xsd:date ;  # Corrected "O3" to "03"
    dcterms:created "2024-02-27"^^xsd:date ;
    dcterms:creator <https://omega-x.eu/> ;
    dcterms:contributor [ foaf:mbox <mailto:bruno.traverson@edf.fr> ; foaf:name "Bruno Traverson" ] ;  # Removed the extra semicolon
    dcterms:contributor [ a foaf:Person ; foaf:name "Maxime Lefrançois" ] ;
    dcterms:license <https://opensource.org/license/mit/> ;
    dcterms:rights "Copyright © Omega-X Consortium 2022-2025"@en ; 
    vann:preferredNamespacePrefix "role" ;
    vann:preferredNamespaceUri <https://w3id.org/omega-x/ontology/EnergyRole/> ;  
    owl:versionIRI <https://w3id.org/omega-x/ontology/EnergyRole-1.0> ;
    owl:versionInfo "1.0" .

#---------------------------------------------------------------
#    Annotation properties
#--------------------------------------------------------------

dcterms:contributor a owl:AnnotationProperty .
dcterms:creator a owl:AnnotationProperty .
dcterms:description a owl:AnnotationProperty .
dcterms:issued a owl:AnnotationProperty .
dcterms:license a owl:AnnotationProperty .
dcterms:modified a owl:AnnotationProperty .
dcterms:title a owl:AnnotationProperty .
vann:preferredNamespacePrefix a owl:AnnotationProperty .
vann:preferredNamespaceUri a owl:AnnotationProperty .
owl:maxQualifiedCardinality a owl:AnnotationProperty .
owl:qualifiedCardinality a owl:AnnotationProperty .

#----------------------------------------------------------------
#    Classes
#----------------------------------------------------------------

#-- Market Participant
role:MarketParticipant a owl:Class ;
        rdfs:label "Market Participant"@en;
	  rdfs:comment "(source IEC 62325-351 Ed.3) The identification of the party participating in energy market business processes."@en ;
        rdfs:isDefinedBy role: .

#-- Market Role
role:MarketRole a owl:Class ;
        rdfs:label "Market Role"@en;
	  rdfs:comment "(source IEC 62325-351 Ed.3) The identification of the intended behaviour of a market participant played within a given business process."@en ;
        rdfs:isDefinedBy role: .

#-- Association
role:Association a owl:Class ;
        rdfs:label "Association"@en;
	  rdfs:comment "(source The PROV Namespace) An instance of prov:Association provides additional descriptions about the binary prov:wasAssociatedWith relation from an prov:Activity to some prov:Agent that had some responsiblity for it."@en ;
        rdfs:seeAlso prov: ;
        rdfs:isDefinedBy role: .

#--------------------------------------------------------------
#    Object Properties
#--------------------------------------------------------------

#-- plays 
role:plays a owl:ObjectProperty ; 
        rdfs:label "has role of"@en ;
        rdfs:comment "(source IEC 62325-351 Ed.3) The role associated with a MarketParticipant."@en;
        owl:inverseOf role:isPlayedBy ;
        rdfs:domain role:MarketParticipant ; 
        rdfs:range role:MarketRole;
        rdfs:isDefinedBy role: .

#-- is played by 
role:isPlayedBy a owl:ObjectProperty ; 
        rdfs:label "is played by"@en ;
        rdfs:comment "(source IEC 62325-351 Ed.3) The participant associated with a MarketRole."@en;
        owl:inverseOf role:hasRoleOf ;
        rdfs:domain role:MarketRole ; 
        rdfs:range role:MarketParticipant ;
        rdfs:isDefinedBy role: .

#-- has role 
role:hasRole a owl:ObjectProperty ; 
        rdfs:label "has role"@en ;
        rdfs:comment "The role part of an Association."@en;
        rdfs:domain role:Association ; 
        rdfs:range role:MarketRole;
        rdfs:isDefinedBy role: .

#-- participant 
role:hasParticipant a owl:ObjectProperty ; 
        rdfs:label "has participant"@en ;
        rdfs:comment "The participant part of an Association."@en;
        rdfs:domain role:Association ; 
        rdfs:range role:MarketParticipant;
        rdfs:isDefinedBy role: .

#-- isAssociatedWith 
role:isAssociatedWith a owl:ObjectProperty ; 
        rdfs:label "is associated with"@en ;
        rdfs:comment "Designates the Market Participant associated."@en;
        rdfs:range role:MarketParticipant;
        rdfs:isDefinedBy role: .

#-- qualifiedAssociation 
role:hasQualifiedAssociation a owl:ObjectProperty ; 
        rdfs:label "has qualified association"@en ;
        rdfs:comment "Designates the Qualified Association concerned."@en;
        rdfs:range role:Association ; 
        rdfs:isDefinedBy role: .

#--------------------------------------------------------------
#    Datatype Properties
#--------------------------------------------------------------

#-- name 
role:name a owl:DatatypeProperty ; 
        rdfs:label "has name"@en ;
        rdfs:comment "the name of a MarketParticipant or of a MarketRole."@en;
        rdfs:range xsd:string ;
        rdfs:isDefinedBy role: .

#-- identifier 
role:identifier a owl:DatatypeProperty ; 
        rdfs:label "has identifier"@en ;
        rdfs:comment "the identifier of a MarketParticipant or of a MarketRole."@en;
        rdfs:range xsd:string ;
        rdfs:isDefinedBy role: .

#----------------------------------------------------------------
#    Taxonomy of Electromobility roles
#----------------------------------------------------------------

#-- Electromobility Market Role
role:ElectromobilityMarketRole a owl:namedIndividual, skos:Concept, role:MarketRole ;
        skos:prefLabel "Electromobility Market Role"@en;
	  skos:definition "The identification of the intended behaviour of an electromobility market participant played within a given business process."@en .

#-- Charge Point Operator
role:ChargePointOperator a owl:namedIndividual, skos:Concept, role:MarketRole ;
        skos:prefLabel "Charge Point Operator"@en;
	  skos:definition "(source OCPI 2.2.1) Abbreviated as CPO. Operates a network of Charge Points."@en ;
        rdfs:seeAlso <https://evroaming.org/app/uploads/2023/12/OCPI-2.2.1-d2-2.pdf> ;
        rdfs:seeAlso uiote:ChargePointOperator .

#-- eMobility Service Provider
role:eMobilityServiceProvider a owl:namedIndividual, skos:Concept, role:MarketRole ;
        skos:prefLabel "eMobility Service Provider"@en;
	  skos:definition "(source OCPI 2.2.1) Abbreviated as eMSP. Gives EV drivers access to charging services."@en ;
        rdfs:seeAlso <https://evroaming.org/app/uploads/2023/12/OCPI-2.2.1-d2-2.pdf> .

#-- eMobility Service Provider for Accessing
role:eMobilityAccessingServiceProvider a  owl:namedIndividual, skos:Concept, role:MarketRole ;
        skos:prefLabel "eMobility Service Provider for Accessing"@en  ;
        skos:definition "The eMobility Service Provider for accessing is a service provider that offers to its end-user-customers the ability of accessing charging services on Charging-Points of a CPO (source eMIP Protocol). "@en .

#-- eMobility Service Provider for Booking
role:eMobilityBookingServiceProvider a  owl:namedIndividual, skos:Concept, role:MarketRole ;
        skos:prefLabel "eMobility Service Provider for Booking"@en  ;
        skos:definition "The eMobility Service Provider for booking is a service provider that offers to its end-user-customer the ability of booking Charging-Points of a CPO (source eMIP Protocol). "@en .

#-- eMobility Service Provider for Roaming
role:eMobilityRoamingServiceProvider a  owl:namedIndividual, skos:Concept, role:MarketRole ;
        skos:prefLabel "eMobility Service Provider for Roaming"@en  ;
        skos:definition "The eMobility Service Provider for roaming is a service provider that facilitates electric vehicle charging access across various networks, enabling seamless charging experiences for drivers while they travel beyond their home network coverage . "@en .

#----------------------------------------------------------------
#    Local Energy Community Classes
#----------------------------------------------------------------

#-- Local Energy Community Market Role
role:LocalEnergyCommunityMarketRole a owl:namedIndividual, skos:Concept, role:MarketRole ;
        skos:prefLabel "Local Energy Community Market Role"@en;
	  skos:definition "The identification of the intended behaviour of a LEC (local energy community) market participant played within a given business process."@en .

#-- Local Energy Community Promoter
role:LocalEnergyCommunityPromoter a owl:namedIndividual, skos:Concept, role:MarketRole ;
        skos:prefLabel "Local Energy Community Promoter"@en;
	  skos:definition "Local Energy Community Promoter."@en .

#----------------------------------------------------------------
#    Flexibility Classes
#----------------------------------------------------------------

#-- Flexibility Market Role
role:FlexibilityMarketRole a owl:namedIndividual, skos:Concept, role:MarketRole ;
        skos:prefLabel "Flexibility Market Role"@en;
	  skos:definition "The identification of the intended behaviour of a flexibility market participant played within a given business process."@en .

#-- Flexibility Provider
role:FlexibilityProvider a owl:namedIndividual, skos:Concept, role:MarketRole ;
        skos:prefLabel "Flexibility Provider"@en;
	  skos:definition "Flexibility Provider."@en .

#-- Flexibility User
role:FlexibilityUser a owl:namedIndividual, skos:Concept, role:MarketRole ;
        skos:prefLabel "Flexibility User"@en;
	  skos:definition "Flexibility User."@en .
