@prefix dcterms: <http://purl.org/dc/terms/> .
@prefix foaf: <http://xmlns.com/foaf/0.1/>.
@prefix geo: <http://www.w3.org/2003/01/geo/wgs84_pos#>.
@prefix infra: <https://w3id.org/omega-x/InfrastructureOntology/>.
@prefix owl: <http://www.w3.org/2002/07/owl#> .
@prefix prop: <https://w3id.org/omega-x/PropertyOntology/>.
@prefix rdf: <http://www.w3.org/1999/02/22-rdf-syntax-ns#> .
@prefix rdfs: <http://www.w3.org/2000/01/rdf-schema#> .
@prefix role: <https://w3id.org/omega-x/EnergyRoleOntology/> .
@prefix sch: <https://schema.org/> .
@prefix seas: <https://w3id.org/seas/> .
@prefix vann: <http://purl.org/vocab/vann/> .
@prefix voaf: <http://purl.org/vocommons/voaf#> .
@prefix vs: <http://www.w3.org/2003/06/sw-vocab-status/ns#> .
@prefix xsd: <http://www.w3.org/2001/XMLSchema#> .

@prefix em: <https://w3id.org/omega-x/ontology/Electromobility/>.
@base  <https://w3id.org/omega-x/ontology/Electromobility/>.

em:ElectromobilityOntology rdf:type owl:Ontology ;
        owl:versionIRI <https://w3id.org/omega-x/ontology/Electromobility-1.1> ;
        dcterms:creator <https://omega-x.eu/>;
	dcterms:contributor[foaf:mbox <mailto:bruno.traverson@edf.fr> ; foaf:name "Bruno Traverson" ;] ;
        dcterms:contributor [a foaf:Person ; foaf:name "Sarra Ben Abbes" ] ;
	dcterms:created "2025-02-05"^^xsd:date ;
        dcterms:rights "Copyright © Omega-X Consortium 2022-2025"@en ;
        dcterms:license <https://www.apache.org/licenses/LICENSE-2.0> ;
	dcterms:modified "2025-02-05"^^xsd:date ;
        dcterms:issued "2025-03-01"^^xsd:date ;
        dcterms:title "Electromobility Ontology"@en ;
        dcterms:description "The Electromobility ontology represents and organizes knowledge about the charging infrastructure for electric vehicles. This ontology defines concepts and relations that are relevant to the charging infrastructure - such as pool, station, charging point and connector- but do not cover electric vehicle characteritics. Roles of stakeholders of the charging infrastructure are further described in the ROLE ontology. Detailed characteristics of charging equipments and sites are given in the PROPERTY module."@en ;
        vann:preferredNamespacePrefix "em" ;
        vann:preferredNamespaceUri <https://w3id.org/omega-x/ElectromobilityOntology/> ;  
	rdfs:label "Electromobility Ontology"@en ;
        owl:versionInfo "1.1" .

#---------------------------------------------------------------
#    Annotation properties
#--------------------------------------------------------------

dcterms:contributor a owl:AnnotationProperty .
dcterms:creator a owl:AnnotationProperty .
dcterms:description a owl:AnnotationProperty .
dcterms:issued a owl:AnnotationProperty .
dcterms:license a owl:AnnotationProperty .
dcterms:modified a owl:AnnotationProperty .
dcterms:title a owl:AnnotationProperty .
foaf:name a owl:DatatypeProperty .
foaf:Person a owl:Class .
vann:preferredNamespacePrefix a owl:AnnotationProperty .
vann:preferredNamespaceUri a owl:AnnotationProperty .
voaf:Vocabulary a owl:Class .
vs:term_status a owl:AnnotationProperty .

#----------------------------------------------------------------
#    Classes
#----------------------------------------------------------------

#-- Electric Vehicle Charging Station Pool
em:ElectricVehicleChargingStationPool a owl:Class ;
	rdfs:label "Electric Vehicle Charging Station Pool"@en;
	rdfs:comment """(source eMIP) A Charging Pool is a location where charging infrastructure elements can be found. A Charging Pool may contain several Charging Stations."""@en ;
        rdfs:seeAlso <https://www.gireve.com/wp-content/uploads/2022/09/Gireve_Tech_eMIP-V0.7.4_ImplementationGuide_1.0.7_en.pdf>;
        rdfs:subClassOf seas:ElectricVehicleChargingStationPool, infra:Site;
        rdfs:isDefinedBy em: .

#-- Equipment
em:Equipment a owl:Class ;
        rdfs:label "Equipment"@en;
	rdfs:comment """Equipmen of Electromobility infratructure. May be either an ElectricVehicleChargingStation, an ElectricVehicleSupplyEquipment or an ElectricVehicleSupplyEquipmentConnector."""@en;
        rdfs:subClassOf infra:Equipment;
        rdfs:isDefinedBy em: .

#-- Electric Vehicle Charging Station
em:ElectricVehicleChargingStation a owl:Class ;
        rdfs:label "Electric Vehicle Charging Station"@en;
	rdfs:comment """(source eMIP) A Charging Station is a physical element, visible for the users, on which Charging Points are available. The Charging Station is also the “Human-Machine Interface” (HMI) between the charge infrastructure and the end users."""@en;
	rdfs:seeAlso <https://www.gireve.com/wp-content/uploads/2022/09/Gireve_Tech_eMIP-V0.7.4_ImplementationGuide_1.0.7_en.pdf>;
        rdfs:subClassOf seas:ElectricVehicleChargingStation, em:Equipment;
        rdfs:isDefinedBy em: .

#-- Electric Vehicle Supply Equipment
em:ElectricVehicleSupplyEquipment a owl:Class ;
        rdfs:label "Electric Vehicle Supply Equipment (EVSE)"@en;
	rdfs:comment """(source eMIP) A Charging Point, synonym of EVSE (Electric Vehicle Supply Equipment), is the energy supply element. An electrical vehicle can connect to a point on one of its connector. A Charging Point may have several Charging Connectors but only one vehicle could be charged at a time on a Charging Point."""@en;
        rdfs:seeAlso <https://www.gireve.com/wp-content/uploads/2022/09/Gireve_Tech_eMIP-V0.7.4_ImplementationGuide_1.0.7_en.pdf>;
        rdfs:subClassOf seas:ElectricVehicleServiceEquipment, em:Equipment;
        rdfs:isDefinedBy em: .

#-- Electric Vehicle Supply Equipment Connector
em:ElectricVehicleSupplyEquipmentConnector a owl:Class ;
        rdfs:label "Electric Vehicle Supply Equipment (EVSE) Connector"@en;
        rdfs:comment """(source eMIP) A Connector related to an Electric Vehicle Supply Equipment (EVSE) that connects to the electric vehicle for the purpose of charging. It is an interface to deliver electricity."""@en ;
        rdfs:seeAlso <https://www.gireve.com/wp-content/uploads/2022/09/Gireve_Tech_eMIP-V0.7.4_ImplementationGuide_1.0.7_en.pdf>;
        rdfs:subClassOf seas:ElectricalConnectionPoint, em:Equipment;
        rdfs:isDefinedBy em: .

#--------------------------------------------------------------
#    Object Properties
#--------------------------------------------------------------

#-- Has Authentication Mode
em:hasAuthenticationMode a owl:ObjectProperty;
	rdfs:label "has authentication mode"@en ;
        rdfs:comment "links an Electric Vehicle Charging Station to its authentication mode."@en ;
        rdfs:domain em:ElectricVehicleChargingStation ;
        rdfs:range prop:AuthenticationMode ;
        rdfs:subPropertyOf infra:hasSystemProperty;
	rdfs:isDefinedBy em: .  

#-- Has Availability Status
em:hasAvailabilityStatus a owl:ObjectProperty;
	rdfs:label "has availability status"@en ;
        rdfs:comment "links an Electric Vehicle Charging Station Pool or an Electromobility Equipment to its availability status."@en ;
        rdfs:range prop:AvailabilityStatus ;
        rdfs:subPropertyOf infra:hasSystemProperty;
        rdfs:isDefinedBy em: .  

#-- Has Charge Point Operator
em:hasChargePointOperator a owl:ObjectProperty;
	rdfs:label "has Charge Point Operator"@en ;
        rdfs:comment "links an Electric Vehicle Charging Station Pool to its charge point operator."@en ;
        rdfs:domain em:ElectricVehicleChargingStationPool ;
        rdfs:range role:MarketParticipant;
        rdfs:subPropertyOf role:isAssociatedWith;
        rdfs:isDefinedBy em: .

#-- Has Charging Speed
em:hasChargingSpeed a owl:ObjectProperty;
	rdfs:label "has Charging Speed"@en ;
        rdfs:comment "links an Electric Vehicle Supply Equipment to its charging speed."@en ;
        rdfs:domain em:ElectricVehicleSupplyEquipment ;
        rdfs:range prop:ChargingSpeed;
        rdfs:subPropertyOf infra:hasSystemProperty;
        rdfs:isDefinedBy em: . 

#-- Has Connector Format 
em:hasConnectorFormat rdf:type owl:ObjectProperty;
        rdfs:label "has connector format"@en ;
	rdfs:comment "links an Electric Vehicle Supply Equipment Connector to its connector format."@en ;
	rdfs:domain em:ElectricVehicleSupplyEquipmentConnector ;
        rdfs:range prop:ElectricVehicleSupplyEquipmentConnectorFormat ;
        rdfs:subPropertyOf infra:hasSystemProperty;
        rdfs:isDefinedBy em: .  

#-- Has Connector Type
em:hasConnectorType rdf:type owl:ObjectProperty;
	rdfs:label "has connector type"@en ;
        rdfs:comment "links an Electric Vehicle Supply Equipment Connector to its connector type."@en ;
        rdfs:domain em:ElectricVehicleSupplyEquipmentConnector ;
        rdfs:range prop:ElectricVehicleSupplyEquipmentConnectorType ;
        rdfs:subPropertyOf infra:hasSystemProperty;
        rdfs:isDefinedBy em: .

#-- Has eMobility Service Provider
em:hasEMobilityServiceProvider a owl:ObjectProperty;
	rdfs:label "has eMobility Service Provider"@en ;
        rdfs:comment "links an Electric Vehicle Charging Station Pool to its eMobility Service Provider."@en ;
        rdfs:domain em:ElectricVehicleChargingStationPool ;
        rdfs:range role:MarketParticipant;
        rdfs:subPropertyOf role:isAssociatedWith;
        rdfs:isDefinedBy em: .

#-- Has Maximum Electric Power
em:hasMaximumElectricPower a owl:ObjectProperty;
	rdfs:label "has maximum electric power"@en ;
        rdfs:comment "links en Electric Vehicle Supply Equipment or Electric Vehicle Supply Equipment Connector to its maximum electric power."@en ;
        rdfs:range prop:Power;
        rdfs:subPropertyOf infra:hasSystemProperty;
        rdfs:isDefinedBy em: .

#-- Has Nominal Power
em:hasNominalPower a owl:ObjectProperty;
	rdfs:label "has nominal power"@en ;
        rdfs:comment "links en Electric Vehicle Supply Equipment or Electric Vehicle Supply Equipment Connector to its nominal power."@en ;
        rdfs:range prop:Power;
        rdfs:subPropertyOf infra:hasSystemProperty;
        rdfs:isDefinedBy em: .

#-- Has Occupancy Status
em:hasOccupancyStatus a owl:ObjectProperty;
	rdfs:label "has occupancy status"@en ;
        rdfs:comment "links an Electric Vehicle Supply Equipment to its occupancy status."@en ;
        rdfs:domain em:ElectricVehicleSupplyEquipment ;
        rdfs:range prop:OccupancyStatus ;
        rdfs:subPropertyOf infra:hasSystemProperty;
        rdfs:isDefinedBy em: .  

#-- Has Payment Method
em:hasPaymentMethod a owl:ObjectProperty;
        rdfs:label "has payment method"@en ;
        rdfs:comment "links an Electric Vehicle Charging Station to its payment method."@en ;
        rdfs:domain em:ElectricVehicleChargingStation ;
        rdfs:range prop:PaymentMethod;
        rdfs:subPropertyOf infra:hasSystemProperty;
        rdfs:isDefinedBy em: .    

#-- Has Power Capability
em:hasPowerCapability a owl:ObjectProperty;
	rdfs:label "has power capability"@en ;
        rdfs:comment "links en Electric Vehicle Supply Equipment or Electric Vehicle Supply Equipment Connector to its power capability."@en ;
        rdfs:range prop:Power;
        rdfs:subPropertyOf infra:hasSystemProperty;
        rdfs:isDefinedBy em: .

#--------------------------------------------------------------
#    Datatype Properties
#--------------------------------------------------------------

#-- Bookable
em:bookable a owl:DatatypeProperty ;       
	rdfs:label "bookable"@en ;
        rdfs:comment "indicates if an Electric Vehicle Supply Equipment can be reserved in advance."@en ;
        rdfs:domain em:ElectricVehicleSupplyEquipment;
	rdfs:range xsd:boolean;
        rdfs:isDefinedBy em: .
 
#-- Name
em:name a owl:DatatypeProperty ;
	rdfs:label "name"@en ;
        rdfs:comment "designates an Electric Vehicle Charging Station Pool."@en ;
	rdfs:domain em:ElectricVehicleChargingStationPool;
	rdfs:range xsd:string;
        rdfs:isDefinedBy em: . 

#-- Visual Identifier
em:visualIdentifier a owl:DatatypeProperty ;
	rdfs:label "visual identifier"@en ;
        rdfs:comment "distinguishes visually an Electromobility Equipment."@en ;
        rdfs:domain em:Equipment;
	rdfs:range xsd:string;
	rdfs:isDefinedBy em: . 
