@prefix omegax: <https://w3id.org/omega-x/ontology> .
@prefix cc: <http://creativecommons.org/ns#> .
@prefix vs: <http://www.w3.org/2003/06/sw-vocab-status/ns#> .
@prefix owl: <http://www.w3.org/2002/07/owl#> .
@prefix rdf: <http://www.w3.org/1999/02/22-rdf-syntax-ns#> .
@prefix xml: <http://www.w3.org/XML/1998/namespace> .
@prefix xsd: <http://www.w3.org/2001/XMLSchema#> .
@prefix foaf: <http://xmlns.com/foaf/0.1/> .
@prefix rdfs: <http://www.w3.org/2000/01/rdf-schema#> .
@prefix vann: <http://purl.org/vocab/vann/> .
@prefix voaf: <http://purl.org/vocommons/voaf#> .
@prefix dcterms: <http://purl.org/dc/terms/> .
@prefix time: <http://www.w3.org/2006/time#> .
@prefix schema: <http://schema.org/>.
@prefix qual: <https://w3id.org/omega-x/ontology/Quality/> .
@prefix prop: <https://w3id.org/omega-x/ontology/Property/> .
@prefix ets: <https://w3id.org/omega-x/ontology/EventsTimeSeries/> .

<https://w3id.org/omega-x/ontology/EventsTimeSeries/> a owl:Ontology ;
                                             owl:versionIRI <https://w3id.org/omega-x/ontology/EventsTimeSeries-1.1/> ;
                                             owl:imports prop: , qual: ;
                                             dcterms:description """ Event and time series ontology describes the global structure of value sets. Value sets can be :
                                                - Data points, elementary data structure that holds a data value and optional data time. 
                                                - Events, elementary data structure that holds an event value and mandatory trigerring time. 
                                                - Data collections, complex data structures that includes multiple data points. 
                                                - Time series, timely ordered data collections. Time series include data points, events or data collections. They can be nested too. 
                                             """@en ;
                                             dcterms:creator <https://omega-x.eu/> ;
                                             dcterms:contributor [a foaf:Person ; foaf:name "Fatma-Zohra Hannou" ] ; 
                                             dcterms:contributor [a foaf:Person ; foaf:name "Lina Nachabe" ] ;
                                             dcterms:contributor [a foaf:Person ; foaf:name "Maxime Lefrançois" ] ;
                                             dcterms:license <https://opensource.org/license/mit/> ;
                                             dcterms:created "2023-11-11"^^xsd:date ;
                                             dcterms:modified "2025-01-14"^^xsd:date;
                                             dcterms:issued "2025-01-30"^^xsd:date;
                                             dcterms:rights "Copyright © Omega-X Consortium 2022-2025"@en ; 
                                             dcterms:title "Event and Time Series ontology"@en ;
                                             vann:preferredNamespacePrefix "ets" ;
                                             vann:preferredNamespaceUri <https://w3id.org/omega-x/ontology/EventsTimeSeries/> ;
                                             rdfs:label "Event and Time Series Ontology"@en ;
                                             owl:versionInfo "1.1".

#---------------------------------------------------------------
#    Annotation properties
#--------------------------------------------------------------

dcterms:contributor a owl:AnnotationProperty .
dcterms:creator a owl:AnnotationProperty .
dcterms:description a owl:AnnotationProperty .
dcterms:issued a owl:AnnotationProperty .
dcterms:license a owl:AnnotationProperty .
dcterms:modified a owl:AnnotationProperty .
dcterms:title a owl:AnnotationProperty .
vann:preferredNamespacePrefix a owl:AnnotationProperty .
vann:preferredNamespaceUri a owl:AnnotationProperty .
owl:maxQualifiedCardinality a owl:AnnotationProperty .
owl:qualifiedCardinality a owl:AnnotationProperty .
vs:term_status a owl:AnnotationProperty .
schema:domainIncludes a owl:AnnotationProperty .
schema:rangeIncludes a owl:AnnotationProperty .
time:TemporalEntity a owl:Class .

#----------------------------------------------------------------
#    Classes
#----------------------------------------------------------------

#--Value Set 
ets:ValueSet rdf:type owl:Class ;
          rdfs:comment "Container for a set of values. The four kinds of value set are: data points, data collections, events and time series."@en ;
          rdfs:label "Value Set"@en ;
          rdfs:subClassOf [ a owl:Restriction ; owl:onProperty ets:hasTemporalContext; owl:someValuesFrom time:TemporalEntity] ;
          rdfs:subClassOf [ a owl:Restriction ; owl:onProperty ets:rank; owl:maxCardinality "1"^^xsd:nonNegativeInteger] ;
          rdfs:subClassOf [ a owl:Restriction ; owl:onProperty ets:creationTime; owl:maxCardinality "1"^^xsd:nonNegativeInteger] ;
          rdfs:subClassOf [ a owl:Restriction ; owl:onProperty ets:isElementOf;  owl:onClass ets:TimeSeries ; owl:maxQualifiedCardinality "1"^^xsd:nonNegativeInteger] .

#--Data Collection
ets:DataCollection a owl:Class ;
        rdfs:subClassOf ets:ValueSet ;
        rdfs:subClassOf [ a owl:Restriction ; owl:onProperty ets:collectionTime ; owl:maxCardinality "1"^^xsd:nonNegativeInteger ] ;
        rdfs:subClassOf [ a owl:Restriction ; owl:onProperty ets:collectionValuesCount;  owl:maxCardinality "1"^^xsd:nonNegativeInteger ] ;
        rdfs:subClassOf [ a owl:Restriction ; owl:onProperty ets:comprises;  owl:minCardinality "1"^^xsd:nonNegativeInteger ] ; 
        rdfs:comment "A data collection represents a set of value sets, that share some common context. Data Collections may also have a common collection time."@en ;
        rdfs:label "Data Collection"@en .

#--Time Series
ets:TimeSeries a owl:Class ;
        rdfs:subClassOf ets:ValueSet ;
        rdfs:subClassOf [ a owl:Restriction ; owl:onProperty ets:hasStep; owl:someValuesFrom time:Duration] ;
        rdfs:subClassOf [ a owl:Restriction ; owl:onProperty ets:seriesElementsCount;  owl:maxCardinality "1"^^xsd:nonNegativeInteger ] ;
        rdfs:subClassOf [ a owl:Restriction ; owl:onProperty ets:isComposedOf;  owl:minCardinality "1"^^xsd:nonNegativeInteger ] ; 
        rdfs:comment "Value container for a time series. Time series elements can be regularly spaced (in time) with a fixed step."@en ;
        rdfs:label "Time Series"@en .

#--Data Point
ets:DataPoint a owl:Class ; 
      rdfs:subClassOf [ a owl:Restriction ; owl:onProperty ets:dataTime ; owl:maxCardinality "1"^^xsd:nonNegativeInteger ] ;
      rdfs:subClassOf [ a owl:Restriction ; owl:onProperty ets:hasDataValue ; owl:cardinality "1"^^xsd:nonNegativeInteger ] ;
      rdfs:subClassOf ets:ValueSet ; 
      rdfs:comment "A data point with possible data time. data points values are provided through Data value instance"@en ; 
      rdfs:label "Data Point"@en ;
      rdfs:isDefinedBy ets:.

#--Event 
ets:Event a owl:Class ;
       rdfs:subClassOf [ a owl:Restriction ; owl:onProperty ets:cause ; owl:maxCardinality "1"^^xsd:nonNegativeInteger ] ;
       rdfs:subClassOf [ a owl:Restriction ; owl:onProperty ets:state ; owl:maxCardinality "1"^^xsd:nonNegativeInteger ] ;
       rdfs:subClassOf [ a owl:Restriction ; owl:onProperty ets:triggeringTime ; owl:maxCardinality "1"^^xsd:nonNegativeInteger ] ;
       rdfs:subClassOf [ a owl:Restriction ; owl:onProperty ets:hasEventValue ; owl:cardinality "1"^^xsd:nonNegativeInteger ] ;
       rdfs:subClassOf ets:ValueSet ;
       rdfs:comment "An occurrence of a change in the environement that happens at a specific time. Event values are provided through data value instance "@en ;
       rdfs:label "Event"@en .

#--Data Value
ets:DataValue a owl:Class ; 
      rdfs:comment "A data value is the entity providing the value of a data point or an event."@en ; 
      rdfs:subClassOf [ a owl:Restriction ; owl:onProperty ets:value ; owl:maxCardinality "1"^^xsd:nonNegativeInteger ] ;
      rdfs:label "Data Value"@en ;
      rdfs:isDefinedBy ets:.

ets:PropertyValue a owl:Class ; rdfs:subClassOf ets:DataValue. 
     
#--------------------------------------------------------------
#    Object Properties
#--------------------------------------------------------------

#--is element of 
ets:isElementOf a owl:ObjectProperty ; 
             owl:inverseOf ets:isComposedOf ;
             rdfs:domain ets:ValueSet ; 
             rdfs:range ets:TimeSeries;
             rdfs:comment "the relationship designating the time series in which the value set is element. A value set can be part of multiple time series."@en;
             rdfs:label "Is Element Of"@en ;
             rdfs:isDefinedBy ets:.

#--is composed of 
ets:isComposedOf a owl:ObjectProperty ;
              owl:inverseOf ets:isElementOf ;
              rdfs:domain ets:TimeSeries ;
              rdfs:range ets:ValueSet ;
              rdfs:comment "the relationship indicating the value sets composing a time series."@en ;
              rdfs:label "is Composed Of"@en ;
              rdfs:isDefinedBy ets:.

#--belongs to
ets:belongsTo a owl:ObjectProperty, owl:FunctionalProperty ; 
             owl:inverseOf ets:comprises ;
             rdfs:domain ets:ValueSet ; 
             rdfs:range ets:DataCollection;
             rdfs:comment "the relationship indicating the data collection to which the value set belongs."@en;
             rdfs:label "Belongs To"@en ;
             rdfs:isDefinedBy ets:.

#--comprises 
ets:comprises a owl:ObjectProperty ;
              owl:inverseOf ets:belongsTo ;
              rdfs:domain ets:DataCollection ;
              rdfs:range ets:ValueSet ;
              rdfs:comment "the relationship indicating value sets comprised in a data collection."@en ;
              rdfs:label "Comprises"@en ;
             rdfs:isDefinedBy ets: .

#--has step
ets:hasStep a owl:ObjectProperty ;
      rdfs:domain ets:TimeSeries ;
      schema:rangeIncludes time:Duration ;
      rdfs:comment "The step between two elements of a time series. This value is only indicated for regular series."@en ;
      rdfs:label "Has Step"@en ;
      rdfs:isDefinedBy ets:.


#--has data value
ets:hasDataValue a owl:ObjectProperty, owl:FunctionalProperty ;
      rdfs:domain ets:DataPoint ;
      rdfs:range ets:DataValue ; 
      rdfs:comment "The relationship indicating a property value for a data point."@en ;
      rdfs:label "Has Data Value"@en .

#--has event value
ets:hasEventValue a owl:ObjectProperty, owl:FunctionalProperty ;
      rdfs:domain ets:Event ;
      rdfs:range ets:DataValue ; 
      rdfs:comment "The relationship indicating a property value for an event."@en ;
      rdfs:label "Has Event Value"@en .

#--has rank property
ets:hasRankProperty a owl:ObjectProperty, owl:FunctionalProperty ;
      rdfs:domain ets:RankDescription ;
      rdfs:range prop:PropertyOfInterest ; 
      rdfs:comment "The relationship identifying the property of interest described by data collections elements sharing the same rank."@en ;
      rdfs:label "Has Rank property"@en .

#--has rank property
ets:hasRankUnit a owl:ObjectProperty, owl:FunctionalProperty ;
      rdfs:domain ets:RankDescription ;
      rdfs:range prop:Unit ; 
      rdfs:comment "The relationship identifying the unit used by values of data collections elements sharing the same rank."@en ;
      rdfs:label "Has Rank Unit"@en .

#--temporal context
ets:hasTemporalContext a owl:ObjectProperty ; 
      rdfs:domain ets:ValueSet ; 
      schema:rangeIncludes time:TemporalEntity ; 
      rdfs:comment "Associates a temporal context for value set coverage. This represents the timeseries entire coverage interval, a data point or an event validity time, i.e time period in which collected values still valid. "@en ; 
      rdfs:label "Has Temporal Context"@en.

#--has Quality Metric
ets:hasQualityMetric a owl:ObjectProperty ; 
      rdfs:domain ets:ValueSet ; 
      rdfs:range qual:QualityMetric ; 
      rdfs:comment "The relationship that indicates a quality metric for the value set "@en ; 
      rdfs:label "Has Quality Metric"@en.

#--has Aggregation Kind
ets:hasAggregationKind a owl:ObjectProperty ; 
      rdfs:domain ets:ValueSet ; 
      rdfs:range qual:Aggregation ; 
      rdfs:comment "The relationship that indicates an aggregation kind for the value set "@en ; 
      rdfs:label "Has Aggregation Kind"@en.

#--is Proided Using
ets:isProvidedUsing a owl:ObjectProperty ; 
      rdfs:domain ets:ValueSet ; 
      rdfs:range qual:MeasuringProcedure ; 
      rdfs:comment "The relationship that indicates a measuring procedure for the value set "@en ; 
      rdfs:label "Is Provided Using"@en.

#--is About Property
ets:isAboutProperty a owl:ObjectProperty ; 
      rdfs:domain ets:ValueSet ; 
      rdfs:range prop:PropertyOfInterest ; 
      rdfs:comment "The relationship that identifies the property of interest described by the value set "@en ; 
      rdfs:label "Is About Property"@en.

ets:allAboutProperty a owl:ObjectProperty ; rdfs:subPropertyOf ets:isAboutProperty; 
      rdfs:domain ets:ValueSet ; 
      rdfs:range prop:PropertyOfInterest ; 
      rdfs:comment "The relationship that identifies the unique property of interest described by the value set "@en ; 
      rdfs:label "All About Property"@en.

ets:someAboutProperty a owl:ObjectProperty ; rdfs:subPropertyOf ets:isAboutProperty; 
      rdfs:domain ets:ValueSet ; 
      rdfs:range prop:PropertyOfInterest ; 
      rdfs:comment "The relationship that identifies one property of interest among those described by the value set "@en ; 
      rdfs:label "Some About Property"@en.

#--has Unit
ets:hasUnit a owl:ObjectProperty ; 
      rdfs:domain ets:ValueSet ; 
      rdfs:range prop:Unit ; 
      rdfs:comment "The relationship that identifies the unit used in the value set"@en ; 
      rdfs:label "Has Unit"@en.

#--------------------------------------------------------------
#    Datatype properties
#---------------------------------------------------------------
#-----Data point datatype properties---
ets:dataTime a owl:DatatypeProperty ;
       rdfs:domain ets:DataPoint;
       rdfs:range xsd:dateTime;
      rdfs:comment "The data time indicating the value recording time."@en ;
      rdfs:label "Data Time"@en ;
             rdfs:isDefinedBy ets:.

#-----Data collection datatype properties---
ets:collectionValuesCount a owl:DatatypeProperty ;
                rdfs:domain ets:DataCollection ;
                rdfs:range xsd:nonNegativeInteger ;
                rdfs:comment "The count of collection data points."@en ;
                rdfs:label "Collection Values Count"@en ;
             rdfs:isDefinedBy ets: .

ets:collectionTime a owl:DatatypeProperty ;
       rdfs:domain ets:DataCollection;
       rdfs:range xsd:dateTime;
      rdfs:comment "The collection time indicating common data points values recording time."@en ;
      rdfs:label "Collection Time"@en ;
      rdfs:isDefinedBy ets: .

#-----Event datatype properties---
ets:cause a owl:DatatypeProperty ;
      rdfs:domain ets:Event;
      schema:rangeIncludes xsd:string ;
      rdfs:comment "The cause that triggered an event."@en ;
      rdfs:label "Cause"@en ;
      rdfs:isDefinedBy ets: .

ets:state a owl:DatatypeProperty ;
      rdfs:domain ets:Event ;
      schema:rangeIncludes xsd:string ;
      rdfs:comment "The state of a system following the occurence of an event."@en ;
      rdfs:label "State"@en ;
      rdfs:isDefinedBy ets:.

ets:triggeringTime a owl:DatatypeProperty ; 
            rdfs:domain ets:Event ; 
            rdfs:range xsd:dateTime ; 
            rdfs:comment "Trigerring time refers to the timestamp when the event occurs in the real world."@en;
            rdfs:label "Triggering Time"@en.

#-----Time Series datatype properties---
ets:seriesElementsCount a owl:DatatypeProperty ;
                rdfs:domain ets:TimeSeries ;
                rdfs:range xsd:nonNegativeInteger ;
                rdfs:comment "The count of timeSeries elements."@en ;
                rdfs:label "Series Elements Count"@en .

#-----ValueSet datatype properties---
ets:rank a owl:DatatypeProperty ;
      rdfs:domain ets:ValueSet;
      rdfs:range xsd:nonNegativeInteger ;
      rdfs:comment "The rank of a value set within a data collection"@en ;
      rdfs:label "Rank"@en ;
      rdfs:isDefinedBy ets:.

ets:name a owl:DatatypeProperty ;
      rdfs:domain ets:ValueSet ;
      rdfs:comment "the name of a value set ."@en ;
      rdfs:label "Name"@en . 

ets:creationTime a owl:DatatypeProperty ; 
            rdfs:domain ets:ValueSet ; 
            rdfs:range xsd:dateTime ; 
            rdfs:comment "Creation time refers to the timestamp when the value set is created."@en;
            rdfs:label "Creation Time"@en.    

#----DataValue datatype properties
ets:value a owl:DatatypeProperty ;  
            rdfs:domain ets:DataValue ;
            rdfs:comment "The value of a data point or an event."@en ;
            rdfs:label "Value"@en .

#----Rank Description datatype properties
ets:describedRank a owl:DatatypeProperty ;  
            rdfs:domain ets:RankDescription ;
            rdfs:range xsd:nonNegativeInteger ;
            rdfs:comment "The described rank refers to the rank of data collcetions described by RankDescription."@en ;
            rdfs:label "Described Rank"@en .
